getSeq

UnitProJ/expressOS/singleLL/MethodsInINode/INode.dfy
@@ -11,14 +11,25 @@ predicate acyclic()
 reads *;
 decreases footprint;
 {
-this in footprint 
-&& (next != null ==> (
-	this !in next.footprint 
+(next == null && footprint == {this}) ||
+(
+(next != null ==> ( this in footprint
+  &&	this !in next.footprint 
   && (( next in footprint &&
 	next.footprint + {this} == footprint && next.acyclic())
 	|| next.Valid())
 	))
-&& forall node :: node in footprint - {this} ==> this !in getFtprint(node)
+&& (forall node :: node in footprint - {this} ==> this !in getFtprint(node))
+)
+
+}
+
+function len():int
+requires Valid();
+reads this, footprint;
+ensures len() == |footprint| == |tailContents| + 1;
+{
+if next == null then 1 else 1 + next.len()
 }
 
 
@@ -122,6 +133,7 @@ this.footprint := {this} + next.footprint;
 
 }
 
+////////////////////////////////////////////////////////
 
 function getFtprint(nd:INode): set<INode>
 reads nd;
@@ -129,61 +141,123 @@ reads nd;
 if nd == null then {} else nd.footprint
 }
 
-
-
-
-/*
-predicate myLemma(nd:INode)
-requires nd != null && nd.acyclic();
-reads *;
-ensures myLemma(nd);
-ensures forall node :: node in nd.footprint - {nd} ==> nd !in getFtprint(node);
+function sumAllFtprint(mySeq: seq<INode>): set<INode>
+reads mySeq;
+ensures forall nd :: nd in mySeq ==> 
+	(nd != null ==> nd.footprint <= sumAllFtprint(mySeq));
 {
-next != null ==> (next.acyclic()
-	|| next.Valid())
+if mySeq == [] then {} else getFtprint(mySeq[0]) + sumAllFtprint(mySeq[1..])
 }
 
-
-function getLen(nd:INode):int
-requires nd != null && nd.acyclic();
-reads *;
-decreases *;
+predicate seqFtprintLemma(mySeq: seq<INode>)
+requires mySeq != [] && null !in mySeq;
+requires forall nd :: nd in mySeq ==> nd.Valid();
+requires forall i :: 0 <= i < |mySeq|-1 ==> mySeq[i].next == mySeq[i+1];
+requires mySeq[|mySeq|-1].next == null;
+reads mySeq, sumAllFtprint(mySeq);
+ensures seqFtprintLemma(mySeq);
+ensures mySeq[0].footprint == (set nd | nd in mySeq);
+ensures forall nd :: nd in mySeq ==> nd.footprint <= mySeq[0].footprint;
+ensures forall nd :: nd in mySeq[1..] ==> nd.footprint < mySeq[0].footprint;
 {
-if nd.next == null then 1 else 1 + getLen(nd.next)
+if |mySeq| == 1 then true
+else (
+mySeq[0].footprint == {mySeq[0]} + mySeq[1].footprint &&
+seqFtprintLemma(mySeq[1..]))
 }
-*/
 
-/*
-function sumAllFtprint(node: INode): set<INode>
-requires node != null ==> node.acyclic();
-reads *;
-decreases footprint + getFtprint(next);
-ensures node != null ==> (forall nd :: nd in node.footprint ==> 
-	(nd != null ==> nd.footprint <= sumAllFtprint(node)));
+predicate seqV(mySeq: seq<INode>)
+requires goodSeqCond(mySeq);
+requires mySeq != [] ==> mySeq[0].Valid();
+
+reads mySeq, sumAllFtprint(mySeq);
+ensures seqV(mySeq);
+ensures goodSeqCond(mySeq);
+ensures forall nd :: nd in mySeq ==> nd.Valid(); 
 {
-if node == null then {} else node.footprint + sumAllFtprint(node.next)
+mySeq == [] ||
+(seqV(mySeq[1..]))
 }
 
 
-ghost method mkValid()
-requires acyclic();
-modifies footprint;
-ensures Valid();
+predicate allNdValid2GoodSeqCond(mySeq: seq<INode>)
+requires seqInv(mySeq);
+requires forall nd :: nd in mySeq ==> nd.Valid();
+requires mySeq != [] ==> mySeq[|mySeq|-1].next == null;
+reads mySeq, sumAllFtprint(mySeq);
+ensures allNdValid2GoodSeqCond(mySeq);
+ensures goodSeqCond(mySeq);
+ensures validSeqCond(mySeq);
 {
-if (next != null)
+if mySeq == [] then true
+else if |mySeq|==1 then mySeq[0].Valid() && mySeq[0].next == null
+else 
+mySeq[0].next == mySeq[1] && seqFtprintLemma(mySeq) &&
+allNdValid2GoodSeqCond(mySeq[1..])
+}
+
+
+predicate goodSeqCond(mySeq: seq<INode>)
+reads mySeq;
 {
-next.mkValid();
-this.tailContents := [next.data] + next.tailContents;
-this.footprint := {this} + next.footprint;
+allDiff(mySeq) &&
+(forall nd :: nd in mySeq ==> nd != null && nd in nd.footprint) &&
+(forall i :: 0 <= i < |mySeq|-1 ==> mySeq[i].next == mySeq[i+1]
+	&& (mySeq != [] ==> mySeq[|mySeq|-1].next !in mySeq)
+	&& mySeq[i].footprint == {mySeq[i]} + mySeq[i+1].footprint) 
+&&(forall i :: 0 <= i < |mySeq| ==> (set nd | nd in mySeq[0..i])					
+				!! mySeq[i].footprint)
 }
 
-else {
-this.tailContents := [];
-this.footprint := {this};
+predicate validSeqCond(mySeq: seq<INode>)
+reads mySeq;
+{
+goodSeqCond(mySeq) &&
+(forall i, j :: 0 <= i < j < |mySeq| ==> 
+	(mySeq[i].footprint > mySeq[j].footprint)) 
+&& (forall nd :: nd in mySeq ==> 
+    (nd.next == null <==> nd == mySeq[|mySeq|-1])
+    && (nd.next != null <==> exists index :: 0 <= index < |mySeq|-1 
+				&& nd == mySeq[index]))
 }
 
+
+//===============================================
+
+predicate allDiff(mySeq:seq<INode>)
+reads mySeq;
+{
+forall index :: 0 <= index < |mySeq| ==> 
+	(forall other :: 0 <= other < |mySeq| && other != index ==>
+	 (mySeq[other] != mySeq[index]))
 }
-*/
+
+
+
+
+
+//==seq invariant inside the loop===
+predicate seqInv(mySeq: seq<INode>)
+reads mySeq;
+{
+allDiff(mySeq) &&
+(forall nd :: nd in mySeq ==> nd != null && nd in nd.footprint) &&
+(forall i :: 0 <= i < |mySeq|-1 ==> mySeq[i].next == mySeq[i+1]) &&
+(mySeq != [] ==> mySeq[|mySeq|-1].next !in mySeq) &&
+(forall i :: 0 <= i < |mySeq| ==> (set nd | nd in mySeq[0..i])					
+				!! mySeq[i].footprint)
+}
+
+
+function getSeq(nd:INode): seq<INode>
+requires nd != null && nd.Valid();
+reads nd, getFtprint(nd);
+ensures forall node :: node in getSeq(nd) ==> node != null && node.Valid();
+//ensures allNdValid2GoodSeqCond(getSeq(nd));
+//ensures validSeqCond(getSeq(nd));
+{
+if nd.next == null then [nd] else [nd] + getSeq(nd.next)
+}
 
 }
 
